extraction/extraction.v
@@ -23,6 +23,8 @@ Require ValueDomain.
 Require Tailcall.
 Require Allocation.
 Require Ctypes.
+Require Csyntax.
+Require Clight.
 Require Compiler.
 Require Parser.
 Require Initializers.
@@ -157,7 +159,8 @@ Cd "extraction".
 Separate Extraction
    Compiler.transf_c_program Compiler.transf_cminor_program
    Cexec.do_initial_state Cexec.do_step Cexec.at_final_state
-   Ctypes.merge_attributes Ctypes.remove_attributes
+   Ctypes.merge_attributes Ctypes.remove_attributes Ctypes.build_composite_env
+   Csyntax.make_program Clight.make_program
    Initializers.transl_init Initializers.constval
    Csyntax.Eindex Csyntax.Epreincr
    Conventions1.dummy_int_reg Conventions1.dummy_float_reg
